Weidenbach_Book/Watched_Literals_Watch_List_Domain.thy
@@ -773,7 +773,6 @@ qed
 lemma in_\<L>\<^sub>a\<^sub>l\<^sub>l_Suc_le_uint_max: \<open>Pos xa \<in># \<L>\<^sub>a\<^sub>l\<^sub>l \<Longrightarrow> Suc xa \<le> uint_max\<close>
   using in_\<L>\<^sub>a\<^sub>l\<^sub>l_less_uint_max by (auto simp: uint_max_def)
 
-
 lemma length_trail_uint_max_div2:
   assumes
     M_\<L>\<^sub>a\<^sub>l\<^sub>l: \<open>\<forall>L\<in>set M. lit_of L \<in># \<L>\<^sub>a\<^sub>l\<^sub>l\<close> and n_d: \<open>no_dup M\<close>
@@ -1028,9 +1027,6 @@ proof -
     unfolding blits_in_\<L>\<^sub>i\<^sub>n_def watched_by.simps
     by blast
 qed
-
-(* TODO Move *)
-(* End Move *)
 
 lemma unit_propagation_inner_loop_body_wl_D_spec:
   fixes S :: \<open>nat twl_st_wl\<close> and K :: \<open>nat literal\<close> and w :: nat
